[Dafny] Use CakeML initial state for top-level compiler proof

compiler/dafny/semantics/dafny_compilerProofScript.sml
@@ -73,30 +73,60 @@ Proof
   \\ irule no_shadow_method_freshen_member \\ simp []
 QED
 
-Triviality has_basic_cons_prim_sem_env:
-  has_basic_cons (SND (THE (prim_sem_env ffi)))
+Definition cml_init_state_def:
+  cml_init_state ffi ck =
+    (FST (THE (prim_sem_env ffi))) with clock := ck
+End
+
+Definition cml_init_env_def:
+  cml_init_env ffi = (SND (THE (prim_sem_env ffi)))
+End
+
+Triviality has_basic_cons_cml_init_env:
+  has_basic_cons (cml_init_env ffi)
 Proof
-  gvs [prim_sem_env_def, prim_types_program_def, add_to_sem_env_def,
-       evaluate_decs_def, check_dup_ctors_def, combine_dec_result_def,
-       has_basic_cons_def, build_tdefs_def, build_constrs_def,
-       extend_dec_env_def]
+  gvs [cml_init_env_def, prim_sem_env_def, prim_types_program_def,
+       add_to_sem_env_def, evaluate_decs_def, check_dup_ctors_def,
+       combine_dec_result_def, has_basic_cons_def, build_tdefs_def,
+       build_constrs_def, extend_dec_env_def]
+QED
+
+Triviality cml_init_state_next_exn_stamp:
+  ExnStamp (cml_init_state ffi ck).next_exn_stamp = ret_stamp
+Proof
+  gvs [cml_init_state_def, prim_sem_env_def, prim_types_program_def,
+       add_to_sem_env_def, evaluate_decs_def, check_dup_ctors_def,
+       combine_dec_result_def, has_basic_cons_def, build_tdefs_def,
+       build_constrs_def, extend_dec_env_def]
+  (* By using rewrite_tac here, we get a more useful proof state (i.e., not just
+     F) if the next extension stamp somehow changes in the future. *)
+  \\ rewrite_tac [ret_stamp_def] \\ simp []
+QED
+
+Triviality cml_init_state_clock:
+  (cml_init_state ffi ck).clock = ck
+Proof
+  gvs [cml_init_state_def]
 QED
 
 Theorem correct_compile:
-  ∀dfy_ck prog s' r_dfy cml_decs ffi (t: 'ffi cml_state).
+  ∀dfy_ck prog s' r_dfy cml_decs (ffi: 'ffi ffi_state).
     evaluate_program dfy_ck T prog = (s', r_dfy) ∧
     compile prog = INR cml_decs ∧ has_main prog ∧ valid_members prog ∧
-    0 < dfy_ck ∧ t.clock = dfy_ck ∧ ExnStamp t.next_exn_stamp = ret_stamp ∧
-    r_dfy ≠ Rstop (Serr Rtype_error) ⇒
+    0 < dfy_ck ∧ r_dfy ≠ Rstop (Serr Rtype_error) ⇒
     ∃ck t' m' r_cml.
-      evaluate_decs (t with clock := t.clock + ck)
-        (SND (THE (prim_sem_env ffi))) cml_decs = (t', r_cml) ∧
-      state_rel m' FEMPTY s' t' (SND (THE (prim_sem_env ffi))) ∧
+      evaluate_decs
+        ((cml_init_state ffi dfy_ck) with
+           clock := (cml_init_state ffi dfy_ck).clock + ck)
+        (cml_init_env ffi) cml_decs = (t', r_cml) ∧
+      state_rel m' FEMPTY s' t' (cml_init_env ffi) ∧
       stmt_res_rel r_dfy r_cml
 Proof
   rpt strip_tac
-  \\ irule correct_from_program
-  \\ irule_at (Pos hd) has_basic_cons_prim_sem_env
+  \\ irule correct_from_program \\ simp []
+  \\ irule_at Any has_basic_cons_cml_init_env
+  \\ irule_at Any cml_init_state_next_exn_stamp
+  \\ simp [cml_init_state_clock]
   \\ fs [compile_def]
   \\ last_assum $ irule_at (Pos last)
   \\ irule_at (Pos last) correct_freshen_program \\ simp []
@@ -106,6 +136,5 @@ Proof
   \\ irule_at (Pos last) map_freshen_member_no_shadow_method
   \\ fs [valid_members_def]
 QED
-
 
 val _ = export_theory ();
